progs/verif_append2.v
@@ -1,27 +1,42 @@
 Require Import VST.floyd.proofauto.
-Require Import VST.floyd.compat.
 Require Import VST.progs.append.
 
 #[export] Instance CompSpecs : compspecs. make_compspecs prog. Defined.
 Definition Vprog : varspecs. mk_varspecs prog. Defined.
 Definition t_struct_list := Tstruct _list noattr.
 
+Lemma not_bot_nonidentity : forall sh,  sh <> Share.bot -> sepalg.nonidentity sh.
+Proof.
+   intros.
+   unfold sepalg.nonidentity. unfold not.
+   intros. apply identity_share_bot in H0. contradiction.   
+Qed.
+Lemma nonidentity_not_bot : forall sh, sepalg.nonidentity sh -> sh <> Share.bot.
+Proof.
+   intros. unfold sepalg.nonidentity. unfold not. intros. apply H. rewrite H0. apply bot_identity.    
+Qed.
+#[export] Hint Resolve not_bot_nonidentity : core.
+#[export] Hint Resolve nonidentity_not_bot : core.
+
+Section Spec.
+
+Context  `{!default_VSTGS Σ}.
 
 Fixpoint listrep (sh: share)
             (contents: list val) (x: val) : mpred :=
  match contents with
  | h::hs =>
-              EX y:val,
-                data_at sh t_struct_list (h,y) x * listrep sh hs y
- | nil => !! (x = nullval) && emp
+              ∃ y:val,
+                data_at sh t_struct_list (h,y) x ∗ listrep sh hs y
+ | nil => ⌜x = nullval⌝ ∧ emp
  end.
 
 Arguments listrep sh contents x : simpl never.
 
 Lemma listrep_local_facts:
   forall sh contents p,
-     listrep sh contents p |--
-     !! (is_pointer_or_null p /\ (p=nullval <-> contents=nil)).
+     listrep sh contents p ⊢
+     ⌜is_pointer_or_null p ∧ (p=nullval <-> contents=nil)⌝.
 Proof.
 intros.
 revert p; induction contents; 
@@ -30,30 +45,28 @@ Intros y. entailer!.
 split; intro. subst p. destruct H; contradiction. inv H2.
 Qed.
 
-#[export] Hint Resolve listrep_local_facts : saturate_local.
+
 
 Lemma listrep_valid_pointer:
   forall sh contents p,
-   sepalg.nonidentity sh ->
-   listrep sh contents p |-- valid_pointer p.
+  sepalg.nonidentity sh ->
+   listrep sh contents p ⊢ valid_pointer p.
 Proof.
  destruct contents; unfold listrep; fold listrep; intros; Intros; subst.
  auto with valid_pointer.
  Intros y.
  apply sepcon_valid_pointer1.
  apply data_at_valid_ptr; auto.
- simpl;  computable.
+ simpl; computable.
 Qed.
 
-#[export] Hint Resolve listrep_valid_pointer : valid_pointer.
-
 Lemma listrep_null: forall sh contents,
-    listrep sh contents nullval = !! (contents=nil) && emp.
+    listrep sh contents nullval ⊣⊢ ⌜contents=nil⌝ ∧ emp.
 Proof.
 destruct contents; unfold listrep; fold listrep.
 autorewrite with norm. auto.
-apply pred_ext.
-Intros y. entailer. destruct H; contradiction.
+apply bi.equiv_entails_2.
+Intros y. entailer!. destruct H; contradiction.
 Intros. discriminate.
 Qed.
 
@@ -73,46 +86,48 @@ Definition append_spec :=
      PARAMS (x; y) GLOBALS()
      SEP (listrep sh s1 x; listrep sh s2 y)
   POST [ tptr t_struct_list ]
-    EX r: val,
+    ∃ r: val,
      PROP()
      RETURN (r)
      SEP (listrep sh (s1++s2) r).
 
 Definition Gprog : funspecs :=   ltac:(with_library prog [ append_spec ]).
 
-Module Proof1.
+Hint Resolve listrep_local_facts : saturate_local.
+Hint Extern 1 (listrep _ _ _ ⊢ valid_pointer _) =>
+    (simple apply listrep_valid_pointer; now auto) : valid_pointer.
 
-Definition lseg (sh: share) (contents: list val) (x z: val) : mpred :=
-  ALL cts2:list val, listrep sh cts2 z -* listrep sh (contents++cts2) x.
+Section Proof1.
 
 Lemma body_append: semax_body Vprog Gprog f_append append_spec.
 Proof.
 start_function.
 forward_if.
 *
- subst x. rewrite listrep_null.  Intros.  subst.
+ subst x.
  forward.
+ rewrite listrep_null. Intros; subst.
  Exists y.
  entailer!!.
  simpl; auto.
 *
  forward.
  destruct s1 as [ | v s1']; unfold listrep at 1; fold listrep.
- Intros.  contradiction.
+ { Intros. contradiction. }
  Intros u.
  remember (v::s1') as s1.
  forward.
  forward_while
-      ( EX a: val, EX s1b: list val, EX t: val, EX u: val,
+      (∃ a: val, ∃ s1b: list val, ∃ t: val, ∃ u: val,
             PROP ()
             LOCAL (temp _x x; temp _t t; temp _u u; temp _y y)
-            SEP (listrep sh (a::s1b++s2) t -* listrep sh (s1++s2) x;
+            SEP (listrep sh (a::s1b++s2) t -∗ listrep sh (s1++s2) x;
                    data_at sh t_struct_list (a,u) t;
                    listrep sh s1b u;
                    listrep sh s2 y))%assert.
 + (* current assertion implies loop invariant *)
    Exists v s1' x u.
-   subst s1. entailer!!. simpl. cancel_wand.
+   entailer!. simpl. cancel_wand.
 + (* loop test is safe to execute *)
    entailer!!.
 + (* loop body preserves invariant *)
@@ -124,14 +139,13 @@ forward_if.
    Exists (v,s1b,u0,z). unfold fst, snd.
    simpl app.
    entailer!!.
-   rewrite sepcon_comm.
-   apply RAMIF_PLAIN.trans''.
-   apply wand_sepcon_adjoint.
-   forget (v::s1b++s2) as s3.
-   unfold listrep; fold listrep; Exists u0; auto.
+   iIntros "[Ha Hb]". iIntros.
+   iApply "Ha".
+   unfold listrep; fold listrep. iExists u0; iFrame.
 + (* after the loop *)
    clear v s1' Heqs1.
    forward.
+   simpl. (* TODO this simpl wasn't needed. maybe store_tac_no_hint in forward1 is broken? *)
    forward.
    rewrite (proj1 H2 (eq_refl _)).
    Exists x.
@@ -139,19 +153,19 @@ forward_if.
    clear.
    entailer!!.
    unfold listrep at 3; fold listrep. Intros.
-   pull_right (listrep sh (a :: s2) t -* listrep sh (s1 ++ s2) x).
-   apply modus_ponens_wand'.
-   unfold listrep at 2; fold listrep. Exists y; cancel.
+   iIntros "(Ha & Hb & Hc & Hd)".
+   iApply "Ha".
+   unfold listrep at -1; fold listrep. iExists y; iFrame.
 Qed.
 
 End Proof1.
 
-Module Proof2.
+Section Proof2.
 
 Definition lseg (sh: share) (contents: list val) (x z: val) : mpred :=
-  ALL cts2:list val, listrep sh cts2 z -* listrep sh (contents++cts2) x.
+  ∀ cts2:list val, listrep sh cts2 z -∗ listrep sh (contents++cts2) x.
 
-Lemma body_append: semax_body Vprog Gprog f_append append_spec.
+Lemma body_append2: semax_body Vprog Gprog f_append append_spec.
 Proof.
 start_function.
 forward_if.
@@ -168,7 +182,7 @@ forward_if.
  remember (v::s1') as s1.
  forward.
  forward_while
-      (EX s1a: list val,  EX a: val, EX s1b: list val, EX t: val, EX u: val,
+      (∃ s1a: list val, ∃ a: val, ∃ s1b: list val, ∃ t: val, ∃ u: val,
             PROP (s1 = s1a ++ a :: s1b)
             LOCAL (temp _x x; temp _t t; temp _u u; temp _y y)
             SEP (lseg sh s1a x t;
@@ -177,7 +191,7 @@ forward_if.
                    listrep sh s2 y))%assert.
 + (* current assertion implies loop invariant *)
    Exists (@nil val) v s1' x u.  entailer!!.
-   unfold lseg. apply allp_right; intro. simpl. cancel_wand.
+   unfold lseg. iIntros. simpl. auto.
 + (* loop test is safe to execute *)
    entailer!!.
 + (* loop body preserves invariant *)
@@ -190,101 +204,93 @@ forward_if.
    rewrite <- !app_assoc. simpl app.
    entailer!!.
    unfold lseg.
-   rewrite sepcon_comm.
+   rewrite bi.sep_comm.
    clear.
-   apply RAMIF_Q.trans'' with (cons a).
-   extensionality cts; simpl; rewrite <- app_assoc; reflexivity.
-   apply allp_right; intro. apply wand_sepcon_adjoint.
-   unfold listrep at 2; fold listrep; Exists u0.  apply derives_refl.
+   iIntros "[H1 H2]".
+   iIntros (cts2) "H3".
+   iSpecialize ("H2" $! (a :: cts2)).
+   rewrite -app_assoc.
+   iApply ("H2").
+   unfold listrep at -1; fold listrep. iExists u0. iFrame.
  + (* after the loop *)
-   forward. forward.
+   forward. simpl. forward.
    Exists x. entailer!!.
    destruct H3 as [? _]. specialize (H3 (eq_refl _)). subst s1b.
    unfold listrep at 1.  Intros. autorewrite with norm.  rewrite H0. rewrite <- app_assoc. simpl app.
    unfold lseg.
-   rewrite sepcon_assoc.
-   eapply derives_trans; [apply allp_sepcon1 | ]. apply allp_left with (a::s2).
-   rewrite sepcon_comm.
-   eapply derives_trans; [ | apply modus_ponens_wand].
-   apply sepcon_derives; [ | apply derives_refl].
-   unfold listrep at 2; fold listrep. Exists y; auto.
+   iIntros "(H1 & H2 & H3)".
+   iApply ("H1" $! (a :: s2)).
+   unfold listrep at 2; fold listrep. iExists y; iFrame.
 Qed.
 
 End Proof2.
 
-Module Proof3.  (*************** inductive lseg *******************)
+Section Proof3.  (*************** inductive lseg *******************)
 
-Fixpoint lseg (sh: share)
+Fixpoint lseg2 (sh: share)
             (contents: list val) (x z: val) : mpred :=
  match contents with
- | h::hs => !! (x<>z) && 
-              EX y:val,
-                data_at sh t_struct_list (h,y) x * lseg sh hs y z
- | nil => !! (x = z /\ is_pointer_or_null x) && emp
+ | h::hs => ⌜x<>z⌝ ∧ 
+              ∃ y:val,
+                data_at sh t_struct_list (h,y) x ∗ lseg2 sh hs y z
+ | nil => ⌜x = z /\ is_pointer_or_null x⌝ ∧ emp
  end.
 
-Arguments lseg sh contents x z : simpl never.
+Arguments lseg2 sh contents x z : simpl never.
+Notation lseg := lseg2.
 
 Lemma lseg_local_facts:
   forall sh contents p q,
-     lseg sh contents p q |--
-     !! (is_pointer_or_null p /\ is_pointer_or_null q /\ (p=q <-> contents=nil)).
+     lseg sh contents p q ⊢
+     ⌜is_pointer_or_null p /\ is_pointer_or_null q /\ (p=q <-> contents=nil)⌝.
 Proof.
 intros.
-apply derives_trans with (lseg sh contents p q && !! (is_pointer_or_null p /\
-        is_pointer_or_null q /\ (p = q <-> contents = []))).
-2: entailer!.
 revert p; induction contents; intros; simpl; unfold lseg; fold lseg.
-entailer!.
-intuition.
-Intros y. Exists y.
-eapply derives_trans.
-apply sepcon_derives.
-apply derives_refl.
-apply IHcontents.
+{ normalize. }
+Intros y.
 entailer!.
 intuition congruence.
 Qed.
 
-#[export] Hint Resolve lseg_local_facts : saturate_local.
+Hint Resolve lseg_local_facts : saturate_local.
 
 Lemma lseg_valid_pointer:
   forall sh contents p ,
    sepalg.nonidentity sh ->
-   lseg sh contents p nullval |-- valid_pointer p.
+   lseg sh contents p nullval ⊢ valid_pointer p.
 Proof.
  destruct contents; unfold lseg; fold lseg; intros. entailer!.
  Intros *.
  auto with valid_pointer.
 Qed.
 
-#[export] Hint Resolve lseg_valid_pointer : valid_pointer.
+Hint Extern 1 (lseg _ _ _ nullval ⊢ valid_pointer _) =>
+    (simple apply lseg_valid_pointer; now auto) : valid_pointer.
 
 Lemma lseg_eq: forall sh contents x,
-    lseg sh contents x x = !! (contents=nil /\ is_pointer_or_null x) && emp.
+    lseg sh contents x x ⊣⊢ ⌜contents=nil /\ is_pointer_or_null x⌝ ∧ emp.
 Proof.
 intros.
 destruct contents; unfold lseg; fold lseg.
-f_equal. f_equal. f_equal. apply prop_ext; intuition.
-apply pred_ext.
-Intros y. contradiction.
-Intros. discriminate.
+- apply and_mono_iff; auto. apply bi.pure_iff. intuition.
+- iSplit. 
+  + iIntros "[%H1 H2]". contradiction.
+  + iIntros "[%H1 H2]". destruct H1. discriminate.
 Qed.
 
 Lemma lseg_null: forall sh contents,
-    lseg sh contents nullval nullval = !! (contents=nil) && emp.
+    lseg sh contents nullval nullval ⊣⊢ ⌜contents=nil⌝ ∧ emp.
 Proof.
 intros.
  rewrite lseg_eq.
- apply pred_ext.
- entailer!.
- entailer!.
+ apply and_mono_iff; auto.
+ apply bi.pure_iff; intuition.
 Qed.
 
-Lemma lseg_cons: forall sh (v u x: val) s,
+Lemma lseg_cons: forall sh (v u x: val) (s: list val),
    readable_share sh ->
- data_at sh t_struct_list (v, u) x * lseg sh s u nullval
- |-- lseg sh [v] x u * lseg sh s u nullval.
+ data_at sh t_struct_list (v, u) x ∗ lseg sh s u nullval
+ ⊢ lseg sh [v] x u ∗ lseg sh s u nullval.
 Proof.
 intros.
      unfold lseg at 2. Exists u. 
@@ -292,20 +298,20 @@ intros.
      destruct s; unfold lseg at 1; fold lseg; entailer.
 Qed.
 
-Lemma lseg_cons': forall sh (v u x a b: val) ,
+Lemma lseg_cons': forall sh (v u x a b: val),
    readable_share sh ->
- data_at sh t_struct_list (v, u) x * data_at sh t_struct_list (a,b) u
- |-- lseg sh [v] x u * data_at sh t_struct_list (a,b) u.
+ data_at sh t_struct_list (v, u) x ∗ data_at sh t_struct_list (a,b) u
+ ⊢ lseg sh [v] x u ∗ data_at sh t_struct_list (a,b) u.
 Proof.
 intros.
-     unfold lseg. Exists u. 
+     unfold lseg. Exists u.
      entailer!.
 Qed.
 
 Lemma lseg_app': forall sh s1 s2 (a w x y z: val),
    readable_share sh ->
-   lseg sh s1 w x * lseg sh s2 x y * data_at sh t_struct_list (a,z) y |--
-   lseg sh (s1++s2) w y * data_at sh t_struct_list (a,z) y.
+   (lseg sh s1 w x ∗ lseg sh s2 x y) ∗ data_at sh t_struct_list (a,z) y ⊢
+   lseg sh (s1++s2) w y ∗ data_at sh t_struct_list (a,z) y.
 Proof.
  intros.
  revert w; induction s1; intro; simpl.
@@ -313,12 +319,12 @@ Proof.
  unfold lseg at 1 3; fold lseg. Intros j; Exists j.
  entailer.
  sep_apply (IHs1 j).
- cancel. 
+ cancel.
 Qed.
-
+ 
 Lemma lseg_app_null: forall sh s1 s2 (w x: val),
    readable_share sh ->
-   lseg sh s1 w x * lseg sh s2 x nullval |--
+   lseg sh s1 w x ∗ lseg sh s2 x nullval ⊢
    lseg sh (s1++s2) w nullval.
 Proof.
  intros.
@@ -332,31 +338,31 @@ Qed.
 
 Lemma lseg_app: forall sh s1 s2 a s3 (w x y z: val),
    readable_share sh ->
-   lseg sh s1 w x * lseg sh s2 x y * lseg sh (a::s3) y z |--
-   lseg sh (s1++s2) w y * lseg sh (a::s3) y z.
+   lseg sh s1 w x ∗ lseg sh s2 x y ∗ lseg sh (a::s3) y z ⊢
+   lseg sh (s1++s2) w y ∗ lseg sh (a::s3) y z.
 Proof.
  intros.
  unfold lseg at 3 5; fold lseg.
- Intros u; Exists u. rewrite prop_true_andp by auto.
+ Intros u; Exists u. rewrite prop_true_andp //.
  sep_apply (lseg_app' sh s1 s2 a w x y u); auto.
  cancel.
 Qed.
 
 Lemma listrep_lseg_null :
- listrep = fun sh s p => lseg sh s p nullval.
+ ∀ sh s p, listrep sh s p ⊣⊢ lseg sh s p nullval.
 Proof.
-extensionality sh s p.
+intros.
 revert p.
 induction s; intros.
-unfold lseg, listrep; apply pred_ext; entailer!.
+unfold lseg, listrep; apply bi.equiv_entails_2; entailer!.
 unfold lseg, listrep; fold lseg; fold listrep.
-apply pred_ext; Intros y; Exists y; rewrite IHs; entailer!.
+apply bi.equiv_entails_2; Intros y; Exists y; rewrite IHs; entailer!.
 Qed.
 
-Lemma body_append: semax_body Vprog Gprog f_append append_spec.
+Lemma body_append3: semax_body Vprog Gprog f_append append_spec.
 Proof.
 start_function.
-revert POSTCONDITION; rewrite listrep_lseg_null; intro.
+rewrite -> listrep_lseg_null in * |- *.
 forward_if.
 *
  subst x. rewrite lseg_null. Intros. subst.
@@ -373,7 +379,7 @@ forward_if.
  remember (v::s1') as s1.
  forward.
  forward_while
-      (EX s1a: list val, EX a: val, EX s1b: list val, EX t: val, EX u: val,
+      (∃ s1a: list val, ∃ a: val, ∃ s1b: list val, ∃ t: val, ∃ u: val,
             PROP (s1 = s1a ++ a :: s1b)
             LOCAL (temp _x x; temp _t t; temp _u u; temp _y y)
             SEP (lseg sh s1a x t; 
@@ -382,7 +388,7 @@ forward_if.
                    lseg sh s2 y nullval))%assert.
  + (* current assertion implies loop invariant *)
      Exists (@nil val) v s1' x u.
-     subst s1. rewrite lseg_eq.
+     subst s1. rewrite lseg_eq listrep_lseg_null.
      entailer.
 (*     sep_apply (lseg_cons sh v u x s1'); auto. *)
  + (* loop test is safe to execute *)
@@ -404,13 +410,14 @@ forward_if.
     subst. rewrite lseg_eq. Intros. subst. 
     forward.
     forward.
-    Exists x. 
+    Exists x.
     entailer!!.
     sep_apply (lseg_cons sh a y t s2); auto.
     sep_apply (lseg_app_null sh [a] s2 t y); auto.
     rewrite <- app_assoc.
     sep_apply (lseg_app_null sh s1a ([a]++s2) x t); auto.
+    rewrite listrep_lseg_null //.
 Qed.
 
 End Proof3.
-
+End Spec.
