progs/io_mem_dry.v
@@ -1,9 +1,9 @@
-Require Import VST.progs64.io_mem_specs.
+Require Import VST.progs.io_mem_specs.
 Require Import VST.floyd.proofauto.
 Require Import VST.sepcomp.extspec.
 Require Import VST.veric.semax_ext.
 Require Import VST.veric.SequentialClight.
-Require Import VST.progs64.dry_mem_lemmas.
+Require Import VST.progs.dry_mem_lemmas.
 Require Import VST.veric.mem_lessdef.
 
 Section IO_Dry.
