progs/verif_bin_search.v
@@ -80,7 +80,7 @@ Qed.
 
 Fixpoint sorted2 l :=
   match l with
-  | [] => True
+  | [] => True%type
   | x :: rest => Forall (fun y => x <= y) rest /\ sorted2 rest
   end.
 
@@ -264,14 +264,13 @@ Definition four_contents := [1; 2; 3; 4].
 Lemma body_main:  semax_body Vprog Gprog f_main main_spec.
 Proof.
   start_function.
+  rename a into gv.
   forward_call (gv _four,Ews,four_contents,3,0,4).
   { change (Zlength four_contents) with 4.
     repeat constructor; computable.
   }
   Intro r; forward.
 Qed.
-
-#[export] Existing Instance NullExtension.Espec.
 
 Lemma prog_correct:
   semax_prog prog tt Vprog Gprog.
