progs/verif_queue2.v
@@ -14,21 +14,21 @@ Definition t_struct_fifo := Tstruct _fifo noattr.
 Proof. eapply mk_listspec; reflexivity. Defined.
 
 Lemma isnil: forall {T: Type} (s: list T), {s=nil}+{s<>nil}.
-Proof. intros. destruct s; [left|right]; auto. intro Hx; inv Hx. Qed.
+Proof. intros. destruct s; [left|right]; auto. Qed.
 
 Lemma field_at_list_cell:
   forall sh i v p,
   data_at sh t_struct_elem (i,v) p
-  = list_cell QS sh i p *
+  ⊣⊢ list_cell QS sh i p *
   field_at sh t_struct_elem [StructField _next] v p.
 Proof.
 intros.
 unfold_data_at (data_at _ _ _ _).
-f_equal.
+f_equiv.
 unfold field_at, list_cell.
 autorewrite with gather_prop.
-f_equal.
-apply ND_prop_ext.
+f_equiv; last done.
+f_equiv.
 rewrite field_compatible_cons; simpl.
 intuition.
 left; auto.
@@ -55,7 +55,7 @@ Definition fifo_body (contents: list val) (hd tl : val) :=
               !!(contents = prefix++last::nil)
             &&  (lseg QS Ews prefix hd tl
                    * malloc_token Ews t_struct_elem tl
-                   * data_at Ews t_struct_elem (last, nullval) tl)))%logic.
+                   * data_at Ews t_struct_elem (last, nullval) tl))).
 
 Definition fifo (contents: list val) (p: val) : mpred :=
   EX ht: (val*val), let (hd,tl) := ht in
@@ -346,8 +346,6 @@ assert_PROP (isptr p3); [entailer! | rewrite if_false by (intro; subst; contradi
 forward. (* return i; *)
 Qed.
 
-#[export] Existing Instance NullExtension.Espec.
-
 Lemma prog_correct:
   semax_prog prog tt Vprog Gprog.
 Proof.
@@ -363,4 +361,3 @@ Proof.
   semax_func_cons body_make_elem.
   semax_func_cons body_main.
 Qed.
-
