progs/verif_sumarray2.v
@@ -125,8 +125,6 @@ forward_call (*  s = sumarray(four+2,2); *)
   forward. (* return *)
 Qed.
 
-#[export] Existing Instance NullExtension.Espec.
-
 Lemma prog_correct:
   semax_prog prog tt Vprog Gprog.
 Proof.
